CCsub_Subcapt.v
@@ -4,44 +4,24 @@ Require Export CCsub_Lemmas.
 
 Local Ltac hint := idtac.
 
-Lemma subcapt_weakening : forall E F G C1 C2,
-  subcapt (G ++ E) C1 C2 ->
-  wf_env (G ++ F ++ E) ->
-  subcapt (G ++ F ++ E) C1 C2.
+Lemma subcapt_weakening : forall Γ Θ Δ C D,
+  (Δ ++ Γ) ⊢ₛ C <: D ->
+  (Δ ++ Θ ++ Γ) ⊢ wf ->
+  (Δ ++ Θ ++ Γ) ⊢ₛ C <: D.
 Proof with eauto using wf_cset_weakening.
   intros * Hsc Hwf.
-  remember (G ++ E).
-  remember (G ++ F ++ E).
-  induction Hsc ; subst...
-  - apply subcapt_universal.
-    + eapply wf_cset_weakening...
-      repeat rewrite dom_concat.
-      fsetdec.
-    + eapply wf_cset_weakening...
-      repeat rewrite dom_concat.
-      fsetdec. 
+  remember (Δ ++ Γ).
+  remember (Δ ++ Θ ++ Γ).
+  induction Hsc; subst...
+  - apply subcapt_universal; eapply wf_cset_weakening...
   - apply subcapt_in...
-    + eapply wf_cset_weakening...
-      repeat rewrite dom_concat.
-      fsetdec.
-    + eapply wf_cset_weakening...
-      repeat rewrite dom_concat.
-      fsetdec.
   - apply subcapt_set...
-    + eapply wf_cset_weakening...
-      repeat rewrite dom_concat.
-      fsetdec.
-    + intros X XNotIn.
-      clear - XNotIn; fsetdec.
-  - eapply subcapt_set...
-    + eapply wf_cset_weakening...
-      repeat rewrite dom_concat.
-      fsetdec.
-    + intros x xIn...
+    intros X XNotIn.
+    apply H1...
 Qed.
 
-Lemma wf_cset_fvarless : forall E A univ,
-  wf_cset E A (cset_set {}A {}N univ).
+Lemma wf_cset_fvarless : forall Γ univ,
+  Γ ⊢ₛ (cset_set {}A {}N univ) wf.
 Proof with eauto.
   intros *.
   constructor...
@@ -52,140 +32,126 @@ Qed.
 
 Hint Resolve wf_cset_fvarless : core.
 
-Lemma subcapt_reflexivity : forall E A C,
-  wf_cset E A C ->
-  A `subset` dom E ->
-  subcapt E C C.
+Lemma subcapt_reflexivity : forall Γ C,
+  Γ ⊢ₛ C wf ->
+  Γ ⊢ₛ C <: C.
 Proof with eauto.
-  intros * WfC HSub.
+  intros * WfC.
   inversion WfC; subst.
   constructor...
-  - eapply wf_cset_set_weakening...
   - intros y yIn.
     apply subcapt_in...
     + apply (wf_cset_singleton_by_mem fvars univ)...
-      eapply wf_cset_set_weakening...
-    + eapply wf_cset_set_weakening... 
   - destruct univ...
 Qed.
 
-Lemma subcapt_transitivity : forall C2 E C1 C3,
-  wf_env E ->
-  subcapt E C1 C2 ->
-  subcapt E C2 C3 ->
-  subcapt E C1 C3.
+Lemma subcapt_transitivity : forall D Γ C E,
+  Γ ⊢ wf ->
+  Γ ⊢ₛ C <: D ->
+  Γ ⊢ₛ D <: E ->
+  Γ ⊢ₛ C <: E.
 Proof with eauto with fsetdec.
-  intros * WfE SC12 SC23.
-  note (wf_cset_in E C3).
-  dependent induction SC12.
-  - inversion SC23; subst.
-    + apply subcapt_universal...
-    + apply subcapt_universal...
-    + assert (univ = true) by csetdec; subst.
-      apply subcapt_universal...
-  - dependent induction SC23.
-    + apply subcapt_universal...
-    + rewrite AtomSetFacts.singleton_iff in H1; symmetry in H1; subst...
-    + exfalso; fsetdec.
+  intros * WfE SCD SDE.
+  note (Γ ⊢ₛ E wf).
+  dependent induction SCD...
+  - Case "subcapt_universal".
+    inversion SDE; subst...
+    assert (univ = true) by csetdec; subst.
+    apply subcapt_universal...
+  - Case "subcapt_in".
+    dependent induction SDE...
     + assert (x = x0) by fsetdec; subst.
       eapply subcapt_var...
     + rewrite AtomSetFacts.singleton_iff in H1; symmetry in H1; subst...
-    + eauto.
-  - dependent induction SC23; eauto using subcapt_universal.
-  - dependent induction SC23; eauto using subcapt_var.
-  - eapply subcapt_tvar with (T := T)...
-  - eapply subcapt_set...
-    + intros ? ?...
-    + destr_bool.
-      inversion SC23; subst...
-      subst...
+  - Case "subcapt_in_univ".
+    dependent induction SDE; eauto using subcapt_universal.
+  - Case "subcapt_var".
+    apply subcapt_set...
+    + intros x xIn.
+      apply H1...
+    + destruct b...
+      destruct univ... 
+      destruct D; simpl in *; subst.
+      inversion SDE...
 Qed.
 
-Lemma subcapt_from_binds : forall P x C E,
-  wf_env E ->
-  binds x (bind_typ (typ_capt C P)) E ->
-  subcapt E (`cset_fvar` x) C.
+Lemma subcapt_from_binds : forall R x C Γ,
+  Γ ⊢ wf ->
+  binds x (bind_typ (C # R)) Γ ->
+  Γ ⊢ₛ (`cset_fvar` x) <: C.
 Proof with eauto.
   intros* ? Binds.
   eapply wf_cset_from_binds in Binds as WfC...
   destruct C...
   eapply wf_typ_from_binds_typ in Binds as WfT...
   inversion WfT;
-    inversion select (wf_cset _ _ _);
+    inversion select (wf_cset _ _);
     subst.
   eapply subcapt_var...
   eapply subcapt_reflexivity...
-  fsetdec.
 Qed.
 
 (* Subtyping implies subcapturing *)
-Lemma sub_implies_subcapt : forall E S T,
-  sub E S T ->
-  subcapt E (cv S) (cv T).
+Lemma sub_implies_subcapt : forall Γ S T,
+  Γ ⊢ S <: T ->
+  Γ ⊢ₛ (typ_cv S) <: (typ_cv T).
 Local Ltac hint ::=
   eauto using subcapt_reflexivity.
 Proof with hint.
   intros * Hsub.
-
-  assert (wf_cset_in E (cv S)); [apply cv_wf|]...
-  assert (wf_cset_in E (cv T)); [apply cv_wf|]...
-  induction Hsub...
-  - eapply subcapt_reflexivity...
-    fsetdec.
-  - eapply subcapt_tvar...
-    apply IHHsub...
-    apply cv_wf.
-    forwards: wf_typ_from_binds_sub H1...
-Qed.
-
-(** TODO: reorganize the contents of the bottom of this file **)
+  assert (Γ ⊢ₛ (typ_cv S) wf); [apply cv_wf|]...
+  assert (Γ ⊢ₛ (typ_cv T) wf); [apply cv_wf|]...
+  induction Hsub; simpl in *...
+  - Case "sub_trans_tvar".
+    apply subcapt_empty...
+  - Case "sub_top".
+    (* REVIEW: not true, this lemma only works for non pure types *)
+    admit.
+Admitted.
 
 (* Substituting the same capture set preserves subcapturing *)
-Lemma subcapt_through_subst_cset : forall x U C F E C1 C2 ,
-  subcapt (F ++ [(x, bind_typ U)] ++ E) C1 C2 ->
-  wf_env (F ++ [(x, bind_typ U)] ++ E) ->
-  subcapt E C (cv U) ->
-  subcapt (map (subst_cb x C) F ++ E) (subst_cset x C C1) (subst_cset x C C2).
+Lemma subcapt_through_subst_cset : forall x U C Δ Γ C1 C2 ,
+  (Δ ++ [(x, bind_typ U)] ++ Γ) ⊢ₛ C1 <: C2 ->
+  (Δ ++ [(x, bind_typ U)] ++ Γ) ⊢ wf ->
+  Γ ⊢ₛ C <: (typ_cv U) ->
+  (map (subst_cb x C) Δ ++ Γ) ⊢ₛ (subst_cset x C C1) <: (subst_cset x C C2).
 Proof with eauto using wf_env_subst_cb, wf_cset_subst_cb with fsetdec.
   intros * Hsc WfE HscC.
   dependent induction Hsc.
-  - assert (wf_cset_in (map (subst_cb x C) F ++ E) (subst_cset x C C0)) as ?WF. {
-      eapply wf_cset_in_subst_cb...
+  - Case "subcapt_universal".
+    assert ((map (subst_cb x C) Δ ++ Γ) ⊢ₛ (subst_cset x C C0) wf) as ?WF. {
+      eapply wf_cset_subst_cb...
     }
-    assert (wf_cset_in (map (subst_cb x C) F ++ E)
-                       (subst_cset x C (cset_set xs {}N true))) as ?WF. {
-      eapply wf_cset_in_subst_cb...
+    assert ((map (subst_cb x C) Δ ++ Γ) ⊢ₛ (subst_cset x C (cset_set xs {}N true)) wf) as ?WF. {
+      eapply wf_cset_subst_cb...
     }
     cbv [subst_cset] in *.
     destruct_set_mem x xs.
-    + assert (wf_typ_in (F ++ [(x, bind_typ U)] ++ E) U) as HA. {
-        note (wf_env ([(x, bind_typ U)] ++ E)) by eauto...
-        rewrite_env (empty ++ (F ++ [(x, bind_typ U)]) ++ E).
-        apply wf_typ_in_weakening; simpl_env...
+    + assert ((Δ ++ [(x, bind_typ U)] ++ Γ) ⊢ U wf) as HA. {
+        note (wf_env ([(x, bind_typ U)] ++ Γ)) by eauto...
+        rewrite_env (∅ ++ (Δ ++ [(x, bind_typ U)]) ++ Γ).
+        apply wf_typ_weakening; simpl_env...
       }
       forwards: cv_wf HA.
-      note (wf_cset_in E C).
-      inversion HA; subst; unfold cset_union; csetsimpl.
-      * unfold cset_union in WF; csetsimpl.
-        apply subcapt_universal...
-      * apply subcapt_universal...
+      note (Γ ⊢ₛ C wf).
+      inversion HA; subst; unfold cset_union; csetsimpl; apply subcapt_universal...
     + apply subcapt_universal...
-  - assert (wf_cset_in (map (subst_cb x C) F ++ E)
-                       (subst_cset x C (cset_set xs {}N b))) as ?WF. {
-      eapply wf_cset_in_subst_cb...
+  - Case "subcapt_in".
+    assert ((map (subst_cb x C) Δ ++ Γ) ⊢ₛ (subst_cset x C (cset_set xs {}N b)) wf) as ?WF. {
+      eapply wf_cset_subst_cb...
     }
-    assert (wf_cset_in (map (subst_cb x C) F ++ E)
-                       (subst_cset x C (`cset_fvar` x0))) as ?WF. {
-      eapply wf_cset_in_subst_cb...
+    assert ((map (subst_cb x C) Δ ++ Γ) ⊢ₛ
+                       (subst_cset x C (`cset_fvar` x0)) wf) as ?WF. {
+      eapply wf_cset_subst_cb...
     }
     unfold subst_cset in *.
     destruct_set_mem x {x0}A.
     + destruct_set_mem x xs.
       2: exfalso; fsetdec.
-      assert (wf_cset_in (F ++ [(x, bind_typ U)] ++ E) C) as HA. {
-        note (wf_env ([(x, bind_typ U)] ++ E)) by eauto...
-        rewrite_env (empty ++ (F ++ [(x, bind_typ U)]) ++ E).
-        apply wf_cset_in_weakening; simpl_env...
+      assert ((Δ ++ [(x, bind_typ U)] ++ Γ) ⊢ₛ C wf) as HA. {
+        note (([(x, bind_typ U)] ++ Γ) ⊢ wf) by eauto...
+        rewrite_env (∅ ++ (Δ ++ [(x, bind_typ U)]) ++ Γ).
+        apply wf_cset_weakening; simpl_env...
       }
       inversion HA; subst.
       csetsimpl.
@@ -199,151 +165,156 @@ Proof with eauto using wf_env_subst_cb, wf_cset_subst_cb with fsetdec.
       2: {
         apply subcapt_in...
       }
-      assert (wf_cset_in (F ++ [(x, bind_typ U)] ++ E) C) as HA. {
-        note (wf_env ([(x, bind_typ U)] ++ E)) by eauto...
-        rewrite_env (empty ++ (F ++ [(x, bind_typ U)]) ++ E).
-        apply wf_cset_in_weakening; simpl_env...
+      assert ((Δ ++ [(x, bind_typ U)] ++ Γ) ⊢ₛ C wf) as HA. {
+        note (([(x, bind_typ U)] ++ Γ) ⊢ wf) by eauto...
+        rewrite_env (∅ ++ (Δ ++ [(x, bind_typ U)]) ++ Γ).
+        apply wf_cset_weakening; simpl_env...
       }
-      note (wf_cset_in E C).
+      note (Γ ⊢ₛ C wf).
       inversion HA; subst.
       csetsimpl.
       apply subcapt_in...
-  - assert (wf_cset_in (map (subst_cb x C) F ++ E) (subst_cset x C D)). {
-      eapply wf_cset_in_subst_cb...
+  - Case "subcapt_in_univ".
+    assert ((map (subst_cb x C) Δ ++ Γ) ⊢ₛ (subst_cset x C D) wf). {
+      eapply wf_cset_subst_cb...
     }
-    inversion select (wf_cset_in _ D); repeat subst. (* so apparently subst isn't idempotent *)
+    inversion select (_ ⊢ₛ D wf); repeat subst. (* so apparently subst isn't idempotent *)
     unfold subst_cset in *.
     find_and_destroy_set_mem; [exfalso;fsetdec|].
     find_and_destroy_set_mem.
-    + note (wf_cset_in E C) by eauto; subst.
+    + note (Γ ⊢ₛ C wf) by eauto; subst.
       csetsimpl.
       apply subcapt_universal...
     + apply subcapt_universal...
-  - unfold subst_cset at 1.
+  - Case "subcapt_var".
+    unfold subst_cset at 1.
     destruct_set_mem x (singleton x0).
     + assert (x0 = x) by fsetdec; subst.
-      assert (binds x (bind_typ U) (F ++ [(x, bind_typ U)] ++ E)) as HA by auto.
+      assert (binds x (bind_typ U) (Δ ++ [(x, bind_typ U)] ++ Γ)) as HA by auto.
       forwards EQ: binds_typ_unique H HA; subst; clear HA.
-      assert (wf_typ_in E U) by eauto.
-      assert (x `notin` dom E) as HA. {
-        assert (ok (F ++ [(x, bind_typ U)] ++ E)) as HA by auto.
+      assert (Γ ⊢ U wf) by eauto.
+      assert (x ∉ dom Γ) as HA. {
+        assert (ok (Δ ++ [(x, bind_typ U)] ++ Γ)) as HA by auto.
         apply ok_tail in HA.
         inversion HA...
       }
       forwards: notin_fv_wf_typ H0 HA.
       replace (C `u` cset_set ({x}A `\`A x) {}N false)
               with C by (destruct U; csetdec).
-      apply (subcapt_transitivity (cv U))... {
-        rewrite_env (empty ++ (map (subst_cb x C) F ++ E)).
+      apply (subcapt_transitivity (typ_cv U))... {
+        rewrite_env (∅ ++ (map (subst_cb x C) Δ ++ Γ)).
         apply subcapt_weakening; simpl_env...
       }
-      replace (cv U) with (subst_cset x C (cv U)).
+      replace (typ_cv U) with (subst_cset x C (typ_cv U)).
       2: {
         symmetry.
         apply subst_cset_fresh.
         destruct U; simpl in *; csetdec.
+        destruct v.
+        - simpl in H2.
+          apply (H1 H2).
+        - simpl in H2.
+          fsetdec. 
       }
       eapply IHHsc...
     + assert (x0 <> x) by fsetdec.
       binds_cases H.
-      * specialize (IHHsc x U F E ltac:(trivial) ltac:(trivial)).
+      * specialize (IHHsc x U Δ Γ ltac:(trivial) ltac:(trivial)).
         forwards: wf_typ_from_binds_typ H...
         eapply subcapt_var with (T := T)...
-        replace (cv T) with (subst_cset x C (cv T)).
+        replace (typ_cv T) with (subst_cset x C (typ_cv T)).
         2: {
           symmetry; apply subst_cset_fresh.
-          assert (x `notin` dom E) as HA. {
-            assert (ok (F ++ [(x, bind_typ U)] ++ E)) as HA by auto.
+          assert (x ∉ dom Γ) as HA. {
+            assert (ok (Δ ++ [(x, bind_typ U)] ++ Γ)) as HA by auto.
             apply ok_tail in HA.
             inversion HA...
           }
           forwards: notin_fv_wf_typ H1 HA.
-          destruct T; simpl in *; fsetdec.
+          destruct T; simpl in *; try fsetdec.
+          destruct v; simpl...
         }
         apply IHHsc...
-      * assert (binds x0 (bind_typ (subst_ct x C T)) (map (subst_cb x C) F ++ E)) as HBnd by auto.
+      * assert (binds x0 (bind_typ (subst_ct x C T)) (map (subst_cb x C) Δ ++ Γ)) as HBnd by auto.
         eapply subcapt_var...
-        replace (cv (subst_ct x C T))
-          with (subst_cset x C (cv T)).
+        replace (typ_cv (subst_ct x C T))
+          with (subst_cset x C (typ_cv T)).
         2: {
-          destruct T; simpl...
-          - unfold subst_cset.
-            destruct_if...
-            exfalso;csetdec.
-          - assert (x <> a). {
-              forwards WfA: wf_typ_from_binds_typ x0 a...
-              assert (binds x _ (F ++ [(x, bind_typ U)] ++ E)) by auto.
-              inversion WfA; subst.
-              forwards: binds_unique a...
-            }
-            unfold subst_cset.
-            destruct_set_mem x {a}A; [exfalso;fsetdec|].
-            easy.
+          destruct T; simpl; unfold subst_cset...
+          destruct v; simpl.
+          2-6: destruct_set_mem x {}A; [ clear - xIn0; exfalso; fsetdec | reflexivity ].
+          assert (x <> a). {
+            forwards WfA: wf_typ_from_binds_typ x0 a...
+            assert (binds x _ (Δ ++ [(x, bind_typ U)] ++ Γ)) by auto.
+            inversion WfA; subst.
+            forwards: binds_unique a...
+          }
+          unfold subst_cset.
+          destruct_set_mem x {a}A; [exfalso;fsetdec|].
+          easy.
         }
         eapply IHHsc...
-
-
-
-
-  - unfold subst_cset at 1.
+  - Case "subcapt_tvar".
+    unfold subst_cset at 1.
     destruct_set_mem x (singleton x0).
     + assert (x0 = x) by fsetdec; subst.
-      assert (binds x (bind_typ U) (F ++ [(x, bind_typ U)] ++ E)) as HA by auto.
+      assert (binds x (bind_typ U) (Δ ++ [(x, bind_typ U)] ++ Γ)) as HA by auto.
       forwards EQ: binds_unique H HA.
       exfalso;congruence.
     + assert (x0 <> x) by fsetdec.
       binds_cases H.
-      * specialize (IHHsc x U F E ltac:(trivial) ltac:(trivial)).
+      * specialize (IHHsc x U Δ Γ ltac:(trivial) ltac:(trivial)).
         forwards: wf_typ_from_binds_sub H...
         eapply subcapt_tvar with (T := T)...
-        replace (cv T) with (subst_cset x C (cv T)).
+        replace (typ_cv T) with (subst_cset x C (typ_cv T)).
         2: {
           symmetry; apply subst_cset_fresh.
-          assert (x `notin` dom E) as HA. {
-            assert (ok (F ++ [(x, bind_typ U)] ++ E)) as HA by auto.
+          assert (x ∉ dom Γ) as HA. {
+            assert (ok (Δ ++ [(x, bind_typ U)] ++ Γ)) as HA by auto.
             apply ok_tail in HA.
             inversion HA...
           }
           forwards: notin_fv_wf_typ H1 HA.
-          destruct T; simpl in *; fsetdec.
+          destruct T; simpl in *; try fsetdec.
+          destruct v; simpl...
         }
         apply IHHsc...
-      * assert (binds x0 (bind_sub (subst_ct x C T)) (map (subst_cb x C) F ++ E)) as HBnd by auto.
+      * assert (binds x0 (bind_sub (subst_ct x C T)) (map (subst_cb x C) Δ ++ Γ)) as HBnd by auto.
         eapply subcapt_tvar...
-        replace (cv (subst_ct x C T)) with (subst_cset x C (cv T)).
+        replace (typ_cv (subst_ct x C T)) with (subst_cset x C (typ_cv T)).
         2: {
-          destruct T; simpl...
-          - unfold subst_cset.
-            destruct_if...
-            exfalso;csetdec.
-          - assert (x <> a). {
-              forwards WfA: wf_typ_from_binds_sub x0 a...
-              assert (binds x _ (F ++ [(x, bind_typ U)] ++ E)) by auto.
-              inversion WfA; subst.
-              forwards: binds_unique a...
-            }
-            unfold subst_cset.
-            destruct_set_mem x {a}A; [exfalso;fsetdec|].
-            easy.
+          destruct T; simpl; unfold subst_cset...
+          destruct v; simpl.
+          2-6: destruct_set_mem x {}A; [ clear - xIn0; exfalso; fsetdec | reflexivity ].
+          assert (x <> a). {
+            forwards WfA: wf_typ_from_binds_sub x0 a...
+            assert (binds x _ (Δ ++ [(x, bind_typ U)] ++ Γ)) by auto.
+            inversion WfA; subst.
+            forwards: binds_unique a...
+          }
+          unfold subst_cset.
+          destruct_set_mem x {a}A; [exfalso;fsetdec|].
+          easy.
         }
         eapply IHHsc...
-  - assert (wf_cset_in (map (subst_cb x C) F ++ E)
-                        (subst_cset x C (cset_set xs {}N b))) as ?WF. {
-      eapply wf_cset_in_subst_cb...
+  - Case "subcapt_set".
+    assert ((map (subst_cb x C) Δ ++ Γ) ⊢ₛ
+                        (subst_cset x C (cset_set xs {}N b)) wf) as ?WF. {
+      eapply wf_cset_subst_cb...
       constructor.
       - intros y yIn.
-        enough (wf_cset_in (F ++ [(x, bind_typ U)] ++ E) (`cset_fvar` y)) as HA. {
+        enough ((Δ ++ [(x, bind_typ U)] ++ Γ) ⊢ₛ (`cset_fvar` y) wf) as HA. {
           inversion HA...
         }
         specialize (H0 y yIn); simpl in H0...
       - intros y yIn.
-        enough (wf_cset_in (F ++ [(x, bind_typ U)] ++ E) (`cset_fvar` y)) as HA. {
+        enough ((Δ ++ [(x, bind_typ U)] ++ Γ) ⊢ₛ (`cset_fvar` y) wf) as HA. {
           inversion HA...
         }
         specialize (H0 y yIn); simpl in H0...
     }
-    assert (wf_cset_in (map (subst_cb x C) F ++ E) (subst_cset x C D)) as ?WF. {
-      eapply wf_cset_in_subst_cb...
+    assert ((map (subst_cb x C) Δ ++ Γ) ⊢ₛ (subst_cset x C D) wf) as ?WF. {
+      eapply wf_cset_subst_cb...
     }
 
     unfold subst_cset at 1.
@@ -363,7 +334,7 @@ Proof with eauto using wf_env_subst_cb, wf_cset_subst_cb with fsetdec.
 
     unfold AtomSet.F.For_all in H0.
     inversion H; subst.
-    note (wf_cset_in E C).
+    note (Γ ⊢ₛ C wf).
 
     rename fvars into cs', univ into b__c', fvars0 into ds, univ0 into b__d.
     unfold subst_cset in WF0 |- *.
@@ -459,13 +430,13 @@ Proof with eauto using wf_env_subst_cb, wf_cset_subst_cb with fsetdec.
         dependent induction H0.
         -- apply subcapt_universal...
            replace (`cset_fvar` y) with (subst_cset x (cset_set ds {}N b__d) (`cset_fvar` y)).
-           eapply wf_cset_in_subst_cb...
+           eapply wf_cset_subst_cb...
            symmetry.
            apply subst_cset_fresh...
         -- cleanup_singleton_eq x y x0 x1.
             apply subcapt_in...
             replace (`cset_fvar` y) with (subst_cset x (cset_set ds {}N b__d) (`cset_fvar` y)).
-            eapply wf_cset_in_subst_cb...
+            eapply wf_cset_subst_cb...
             symmetry.
             apply subst_cset_fresh...
         -- cleanup_singleton_eq x y x0 x1.
@@ -512,7 +483,7 @@ Proof with eauto using wf_env_subst_cb, wf_cset_subst_cb with fsetdec.
       * destruct_union_mem yIn.
         2: exfalso...
         rename H1 into H1'.
-        forwards H1: (>> H1' x xIn x U F E)...
+        forwards H1: (>> H1' x xIn x U Δ Γ)...
         move H1 before H1'; clear H1'.
         unfold subst_cset at 1 in H1.
         destruct_set_mem x {x}A; [|exfalso;fsetdec].
@@ -524,19 +495,19 @@ Proof with eauto using wf_env_subst_cb, wf_cset_subst_cb with fsetdec.
 
         replace (ds `u`A {x}A `\`A x) with ds in H1 by fsetdec.
 
-        enough (subcapt (map (subst_cb x (cset_set ds {}N b__d)) F ++ E)
+        enough (subcapt (map (subst_cb x (cset_set ds {}N b__d)) Δ ++ Γ)
                           (`cset_fvar` y)
                           (cset_set ds {}N b__d)) as HAA. {
           eapply subcapt_transitivity...
         }
         eapply subcapt_in...
-        admit.
-Admitted.
+        eapply wf_cset_singleton_by_mem...
+Qed.
 
-Lemma wf_cset_atom_union : forall E A xs ys u1 u2,
-  wf_cset E A (cset_set xs {}N u1) ->
-  wf_cset E A (cset_set ys {}N u2) ->
-  wf_cset E A (cset_set (xs `union` ys) {}N (u1 || u2)).
+Lemma wf_cset_atom_union : forall Γ xs ys u1 u2,
+  Γ ⊢ₛ (cset_set xs {}N u1) wf ->
+  Γ ⊢ₛ (cset_set ys {}N u2) wf ->
+  Γ ⊢ₛ (cset_set (xs `union` ys) {}N (u1 || u2)) wf.
 Proof with eauto.
   intros * WfXs WfYs.
   inversion WfXs; inversion WfYs; subst.
@@ -547,10 +518,10 @@ Proof with eauto.
   fsetdec.
 Qed.
 
-Lemma subcapt_expansion : forall E C D1 D2,
-  wf_cset_in E D2 ->
-  subcapt E C D1 ->
-  subcapt E C (cset_union D1 D2).
+Lemma subcapt_expansion : forall Γ C D1 D2,
+  Γ ⊢ₛ D2 wf ->
+  Γ ⊢ₛ C <: D1 ->
+  Γ ⊢ₛ C <: (D1 `u` D2).
 Proof with eauto using wf_cset_union, wf_cset_atom_union with fsetdec.
   intros * HwfD2 Hsubcapt.
   induction Hsubcapt.
@@ -581,35 +552,33 @@ Tactic Notation "subst_mem_singleton" "<-" hyp(H) :=
     | _ `in`A _ => rewrite AtomSetFacts.singleton_iff in H; symmetry in H; subst
   end.
 
-Lemma subcapt_singleton_mem: forall x E C D,
-  wf_env E ->
-  subcapt E C D ->
+Lemma subcapt_singleton_mem: forall x Γ C D,
+  Γ ⊢ wf ->
+  Γ ⊢ₛ C <: D ->
   x A`in` C ->
-  subcapt E (`cset_fvar` x) D.
+  Γ ⊢ₛ (`cset_fvar` x) <: D.
 Proof with eauto with fsetdec.
-  intros * WfE Hsc xIn.
+  intros * WfΓ Hsc xIn.
   dependent induction Hsc...
   - apply subcapt_universal...
-    note (wf_cset_in E C).
+    note (Γ ⊢ₛ C wf).
     eapply wf_cset_singleton_by_mem...
   - eapply subcapt_in...
     replace x with x0 by (clear - xIn; fsetdec)...
   - clear - xIn; fsetdec.
   - subst_mem_singleton xIn.
-    apply (subcapt_transitivity (cv T))...
+    apply (subcapt_transitivity (typ_cv T))...
     eapply subcapt_var...
     eapply subcapt_reflexivity...
-    fsetdec.
   - subst_mem_singleton xIn.
-    apply (subcapt_transitivity (cv T))...
+    apply (subcapt_transitivity (typ_cv T))...
     eapply subcapt_tvar...
     eapply subcapt_reflexivity...
-    fsetdec.
 Qed.
 
-Lemma subcapt_universal_mem: forall E C D,
-  wf_env E ->
-  subcapt E C D ->
+Lemma subcapt_universal_mem: forall Γ C D,
+  Γ ⊢ wf ->
+  Γ ⊢ₛ C <: D ->
   implb (`cset_uvar` C) (`cset_uvar` D) = true.
 Proof with eauto with fsetdec.
   intros * WfE Hsc.
@@ -617,17 +586,17 @@ Proof with eauto with fsetdec.
   csetdec.
 Qed.
 
-Lemma subcapt_union_distributivity : forall E C1 C2 D,
-  wf_env E ->
-  subcapt E C1 D ->
-  subcapt E C2 D ->
-  subcapt E (cset_union C1 C2) D.
+Lemma subcapt_union_distributivity : forall Γ C1 C2 D,
+  Γ ⊢ wf ->
+  Γ ⊢ₛ C1 <: D ->
+  Γ ⊢ₛ C2 <: D ->
+  Γ ⊢ₛ (C1 `u` C2) <: D.
 Proof with eauto using wf_cset_union with fsetdec.
-  intros * WfE HscC1 HscC2.
-  assert (wf_cset_in E (cset_union C1 C2)) by auto using wf_cset_union.
+  intros * WfΓ HscC1 HscC2.
+  assert (Γ ⊢ₛ (C1 `u` C2) wf) by auto using wf_cset_union.
   generalize dependent C2.
   dependent induction HscC1; intros C2 HscC2 WF__union...
-  - note (wf_cset_in E C2); csetsimpl.
+  - note (Γ ⊢ₛ C2 wf); csetsimpl.
     apply subcapt_set.
     + trivial...
     + intros y yIn.
@@ -637,21 +606,23 @@ Proof with eauto using wf_cset_union with fsetdec.
       * applys subcapt_transitivity HscC2...
         apply subcapt_in...
         apply wf_concrete_cset...
-        fsetdec.
+        2: fsetdec.
+        intros z zIn...
     + forwards: subcapt_universal_mem HscC2...
-  - note (wf_cset_in E C2); csetsimpl.
+  - note (Γ ⊢ₛ C2 wf); csetsimpl.
     apply subcapt_set.
     + trivial...
     + intros y yIn.
       applys subcapt_transitivity HscC2...
       apply subcapt_in...
       apply wf_concrete_cset...
-      fsetdec.
+      2: fsetdec.
+      intros z zIn...
     + forwards: subcapt_universal_mem HscC2...
-  - apply (subcapt_transitivity (cv T `u` C2))...
-    assert (wf_cset_in E (cv T `u` C2)) as WfU by auto using wf_cset_union.
-    note (wf_cset_in E C2).
-    note (wf_cset_in E (cv T)).
+  - apply (subcapt_transitivity (typ_cv T `u` C2))...
+    assert (Γ ⊢ₛ (typ_cv T `u` C2) wf) as WfU by auto using wf_cset_union.
+    note (Γ ⊢ₛ C2 wf).
+    note (Γ ⊢ₛ (typ_cv T) wf).
     rewrite <- H2 in WfU.
     csetsimpl.
     apply subcapt_set...
@@ -659,24 +630,25 @@ Proof with eauto using wf_cset_union with fsetdec.
     intros y yIn.
     destruct_union_mem yIn.
     + subst_mem_singleton yIn.
-      apply (subcapt_transitivity (cv T))...
+      apply (subcapt_transitivity (typ_cv T))...
       * eapply subcapt_var...
         eapply subcapt_reflexivity...
-        fsetdec.
       * rewrite <- H2.
         apply subcapt_set...
         2: csetdec.
         intros z zIn.
         apply subcapt_in...
         apply wf_concrete_cset...
-        fsetdec.
+        2: fsetdec.
+        intros w wIn...
     + apply subcapt_in...
       apply wf_concrete_cset...
-      fsetdec.
-  - apply (subcapt_transitivity (cv T `u` C2))...
-    assert (wf_cset_in E (cv T `u` C2)) as WfU by auto using wf_cset_union.
-    note (wf_cset_in E C2).
-    note (wf_cset_in E (cv T)).
+      2: fsetdec.
+      intros z zIn...
+  - apply (subcapt_transitivity (typ_cv T `u` C2))...
+    assert (Γ ⊢ₛ (typ_cv T `u` C2) wf) as WfU by auto using wf_cset_union.
+    note (Γ ⊢ₛ C2 wf).
+    note (Γ ⊢ₛ (typ_cv T) wf).
     rewrite <- H2 in WfU.
     csetsimpl.
     apply subcapt_set...
@@ -684,93 +656,99 @@ Proof with eauto using wf_cset_union with fsetdec.
     intros y yIn.
     destruct_union_mem yIn.
     + subst_mem_singleton yIn.
-      apply (subcapt_transitivity (cv T))...
+      apply (subcapt_transitivity (typ_cv T))...
       * eapply subcapt_tvar...
         eapply subcapt_reflexivity...
-        fsetdec.
       * rewrite <- H2.
         apply subcapt_set...
         2: csetdec.
         intros z zIn.
         apply subcapt_in...
         apply wf_concrete_cset...
-        fsetdec.
+        2: fsetdec.
+        intros w wIn...
     + apply subcapt_in...
       apply wf_concrete_cset...
-      fsetdec.
-  - note (wf_cset_in E C2); csetsimpl.
+      2: fsetdec.
+      intros z zIn...
+  - note (Γ ⊢ₛ C2 wf); csetsimpl.
     apply subcapt_set...
     + intros y yIn.
       destruct_union_mem yIn...
       apply (subcapt_transitivity (cset_set fvars {}N univ))...
       eapply subcapt_in...
       apply wf_concrete_cset...
-      fsetdec.
+      2: fsetdec.
+      intros z zIn...
     + forwards: subcapt_universal_mem HscC2; csetdec...
 Qed.
 
 Lemma cset_union_symmetrical : forall C D,
-  cset_union C D = cset_union D C.
+  C `u` D = D `u` C.
 Proof with eauto.
   intros.
   destruct C; destruct D; simpl; try easy.
   csetdec.
 Qed.
 
-Lemma union_under_subcapturing : forall E C1 C2 D1 D2,
-  wf_env E ->
-  subcapt E C1 C2 ->
-  subcapt E D1 D2 ->
-  subcapt E (cset_union C1 D1) (cset_union C2 D2).
+Lemma union_under_subcapturing : forall Γ C1 C2 D1 D2,
+  Γ ⊢ wf ->
+  Γ ⊢ₛ C1 <: C2 ->
+  Γ ⊢ₛ D1 <: D2 ->
+  Γ ⊢ₛ (C1 `u` D1) <: (C2 `u` D2).
 Proof with eauto.
-  intros * WfE Hsc1 Hsc2.
+  intros * WfΓ Hsc1 Hsc2.
   apply subcapt_union_distributivity...
   - apply subcapt_expansion...
   - rewrite cset_union_symmetrical.
     apply subcapt_expansion...
 Qed.
 
-Lemma subcapt_through_subst_tt : forall E P Q F X C D,
-  wf_env (F ++ [(X, bind_sub Q)] ++ E) ->
-  subcapt (F ++ [(X, bind_sub Q)] ++ E) C D ->
-  sub E P Q ->
-  subcapt (map (subst_tb X P) F ++ E) (subst_cset X (cv P) C) (subst_cset X (cv P) D).
-Proof with eauto using wf_env_subst_tb, wf_cset_in_subst_tb, wf_typ_in_subst_tb with fsetdec.
+Lemma subcapt_through_subst_tt : forall Γ P Q Δ X C D,
+  (Δ ++ [(X, bind_sub Q)] ++ Γ) ⊢ wf ->
+  (Δ ++ [(X, bind_sub Q)] ++ Γ) ⊢ₛ C <: D ->
+  (* TODO:
+      Q pure from wf_env
+      Q pure and P <: Q => P pure
+  *)
+  Γ ⊢ P <: Q ->
+  (map (subst_tb X P) Δ ++ Γ) ⊢ₛ (subst_cset X (typ_cv P) C) <: (subst_cset X (typ_cv P) D).
+Proof with eauto using wf_env_subst_tb, wf_cset_subst_tb, wf_typ_subst_tb with fsetdec.
   intros * Hwf Hsc Hsub.
+  assert ((map (subst_tb X P) Δ ++ Γ) ⊢ wf).
+  { eapply wf_env_subst_tb...
+    admit.
+  }
   generalize dependent P.
-  dependent induction Hsc; intros P Hsub.
-  - assert (wf_cset_in (map (subst_tb X P) F ++ E) (subst_cset X (cv P) C)) as ?WF...
-    assert (wf_cset_in (map (subst_tb X P) F ++ E)
-                       (subst_cset X (cv P) (cset_set xs {}N true))) as ?WF...
+  dependent induction Hsc; intros P Hsub Henv.
+  - assert ((map (subst_tb X P) Δ ++ Γ) ⊢ₛ (subst_cset X (typ_cv P) C) wf) as ?WF...
+    assert ((map (subst_tb X P) Δ ++ Γ) ⊢ₛ
+                       (subst_cset X (typ_cv P) (cset_set xs {}N true)) wf) as ?WF...
     cbv [subst_cset] in *.
     destruct_set_mem X xs.
-    + assert (wf_typ_in (F ++ [(X, bind_sub Q)] ++ E) P) as HA. {
-        note (wf_env ([(X, bind_sub Q)] ++ E)) by eauto...
-        rewrite_env (empty ++ (F ++ [(X, bind_sub Q)]) ++ E).
-        apply wf_typ_in_weakening; simpl_env...
+    + assert ((Δ ++ [(X, bind_sub Q)] ++ Γ) ⊢ P wf) as HA. {
+        note (([(X, bind_sub Q)] ++ Γ) ⊢ wf) by eauto...
+        rewrite_env (∅ ++ (Δ ++ [(X, bind_sub Q)]) ++ Γ).
+        apply wf_typ_weakening; simpl_env...
       }
       forwards: cv_wf HA.
-      inversion HA; subst; simpl.
-      * simpl in *; csetsimpl.
-        apply subcapt_universal...
-      * simpl in *; csetsimpl.
-        apply subcapt_universal...
+      inversion HA; subst; simpl in *; csetsimpl; apply subcapt_universal...
     + apply subcapt_universal...
-  - assert (wf_cset_in (map (subst_tb X P) F ++ E) (subst_cset X (cv P) (`cset_fvar` x))) as ?WF...
-    assert (wf_cset_in (map (subst_tb X P) F ++ E)
-                       (subst_cset X (cv P) (cset_set xs {}N b))) as ?WF...
+  - assert ((map (subst_tb X P) Δ ++ Γ) ⊢ₛ (subst_cset X (typ_cv P) (`cset_fvar` x)) wf) as ?WF...
+    assert ((map (subst_tb X P) Δ ++ Γ) ⊢ₛ
+                       (subst_cset X (typ_cv P) (cset_set xs {}N b)) wf) as ?WF...
     unfold subst_cset in *.
     destruct_set_mem X {x}A.
     + destruct_set_mem X xs.
       2: exfalso; fsetdec.
-      assert (wf_cset_in (F ++ [(X, bind_sub Q)] ++ E) (cv P)) as HA. {
-        note (wf_env ([(X, bind_sub Q)] ++ E)) by eauto...
-        rewrite_env (empty ++ (F ++ [(X, bind_sub Q)]) ++ E).
-        apply wf_cset_in_weakening; simpl_env; [apply cv_wf|]...
+      assert ((Δ ++ [(X, bind_sub Q)] ++ Γ) ⊢ₛ (typ_cv P) wf) as HA. {
+        note (([(X, bind_sub Q)] ++ Γ) ⊢ wf) by eauto...
+        rewrite_env (∅ ++ (Δ ++ [(X, bind_sub Q)]) ++ Γ).
+        apply wf_cset_weakening; simpl_env; [apply cv_wf|]...
       }
       inversion HA; subst; csetsimpl.
       replace (xs `union` singleton x `remove` X) with xs by fsetdec.
-      rename select (_ = cv P) into EQ.
+      rename select (_ = typ_cv P) into EQ.
       rewrite <- EQ in WF0; csetsimpl in WF0.
       apply subcapt_set...
       * intros y yIn.
@@ -781,24 +759,24 @@ Proof with eauto using wf_env_subst_tb, wf_cset_in_subst_tb, wf_typ_in_subst_tb 
       2: {
         apply subcapt_in...
       }
-      assert (wf_cset_in (F ++ [(X, bind_sub Q)] ++ E) (cv P)) as HA. {
-        note (wf_env ([(X, bind_sub Q)] ++ E)) by eauto...
-        rewrite_env (empty ++ (F ++ [(X, bind_sub Q)]) ++ E).
-        apply wf_cset_in_weakening; simpl_env; [apply cv_wf|]...
+      assert ((Δ ++ [(X, bind_sub Q)] ++ Γ) ⊢ₛ (typ_cv P) wf) as HA. {
+        note (([(X, bind_sub Q)] ++ Γ) ⊢ wf) by eauto...
+        rewrite_env (∅ ++ (Δ ++ [(X, bind_sub Q)]) ++ Γ).
+        apply wf_cset_weakening; simpl_env; [apply cv_wf|]...
       }
       inversion HA; subst; csetsimpl.
-      rename select (_ = cv P) into EQ.
+      rename select (_ = typ_cv P) into EQ.
       rewrite <- EQ in WF0; csetsimpl in WF0.
       apply subcapt_in...
-  - assert (wf_cset_in (map (subst_tb X P) F ++ E) (subst_cset X (cv P) D))...
-    inversion select (wf_cset_in _ D); repeat subst. (* so apparently subst isn't idempotent *)
+  - assert ((map (subst_tb X P) Δ ++ Γ) ⊢ₛ (subst_cset X (typ_cv P) D) wf)...
+    inversion select (_ ⊢ₛ D wf); repeat subst. (* so apparently subst isn't idempotent *)
     unfold subst_cset in *.
     find_and_destroy_set_mem; [exfalso;fsetdec|].
     find_and_destroy_set_mem.
-    + assert (wf_cset_in E (cv P)) as HA; [|inversion HA; subst]. {
+    + assert (Γ ⊢ₛ (typ_cv P) wf) as HA; [|inversion HA; subst]. {
         apply cv_wf...
       }
-      rename select (_ = cv P) into EQ.
+      rename select (_ = typ_cv P) into EQ.
       rewrite <- EQ in H1.
       csetsimpl.
       apply subcapt_universal...
@@ -806,122 +784,121 @@ Proof with eauto using wf_env_subst_tb, wf_cset_in_subst_tb, wf_typ_in_subst_tb 
   - unfold subst_cset at 1.
     destruct_set_mem X {x}A.
     + assert (x = X) by fsetdec; subst.
-      assert (binds X (bind_sub Q) (F ++ [(X, bind_sub Q)] ++ E)) as HA by auto.
+      assert (binds X (bind_sub Q) (Δ ++ [(X, bind_sub Q)] ++ Γ)) as HA by auto.
       forwards: binds_unique (bind_typ T) (bind_sub Q)...
       congruence.
     + assert (x <> X) by fsetdec.
       binds_cases H.
-      * specialize (IHHsc X F Q E ltac:(trivial) ltac:(trivial) ltac:(trivial)).
+      * specialize (IHHsc X Δ Q Γ ltac:(trivial) ltac:(trivial) ltac:(trivial)).
         forwards: wf_typ_from_binds_typ H...
         eapply subcapt_var with (T := T)...
-        replace (cv T) with (subst_cset X (cv P) (cv T)).
+        replace (typ_cv T) with (subst_cset X (typ_cv P) (typ_cv T)).
         2: {
           symmetry; apply subst_cset_fresh.
-          assert (X `notin` dom E) as HA. {
-            assert (ok (F ++ [(X, bind_sub Q)] ++ E)) as HA by auto.
+          assert (X ∉ dom Γ) as HA. {
+            assert (ok (Δ ++ [(X, bind_sub Q)] ++ Γ)) as HA by auto.
             apply ok_tail in HA.
             inversion HA...
           }
           forwards: notin_fv_wf_typ H1 HA.
-          destruct T; simpl in *; fsetdec.
+          destruct T; simpl in *; try fsetdec.
+          destruct v...
         }
         apply IHHsc...
-      * assert (binds x (bind_typ (subst_tt X P T)) (map (subst_tb X P) F ++ E)) as HBnd by auto.
+      * assert (binds x (bind_typ (subst_tt X P T)) (map (subst_tb X P) Δ ++ Γ)) as HBnd by auto.
         eapply subcapt_var...
-        replace (cv (subst_tt X P T))
-          with (subst_cset X (cv P) (cv T)).
+        replace (typ_cv (subst_tt X P T))
+          with (subst_cset X (typ_cv P) (typ_cv T)).
         1: eapply IHHsc...
         1: {
-          destruct T; simpl...
-          - unfold subst_cset.
-            destruct_if...
-            exfalso;csetdec.
-          - unfold subst_cset.
-            destruct (a == X); destruct_set_mem X {a}A; try (exfalso;fsetdec).
-            2: simpl...
-            note (wf_typ_in E P); simpl; unfold cset_union; csetdec.
+          destruct T; unfold subst_cset; simpl...
+          destruct v; simpl...
+          2-6: destruct_if; [ exfalso; csetdec | reflexivity ].
+          destruct (a == X); destruct_set_mem X {a}A; try (exfalso;fsetdec).
+          2: simpl...
+          note (Γ ⊢ P wf); simpl; unfold cset_union; csetdec.
         }
   - unfold subst_cset at 1.
     destruct_set_mem X (singleton x).
     + assert (x = X) by fsetdec; subst.
-      assert (binds X (bind_sub Q) (F ++ [(X, bind_sub Q)] ++ E)) as HBnd by auto.
+      assert (binds X (bind_sub Q) (Δ ++ [(X, bind_sub Q)] ++ Γ)) as HBnd by auto.
       forwards EQ: binds_unique H HBnd.
       inversion EQ; subst.
-      assert (wf_typ_in E P) as WfP by eauto.
-      assert (wf_typ_in E Q) as WfQ by eauto.
-      assert (X `notin` dom E) as HA. {
-        assert (ok (F ++ [(X, bind_sub Q)] ++ E)) as HA by auto.
+      assert (Γ ⊢ P wf) as WfP by eauto.
+      assert (Γ ⊢ Q wf) as WfQ by eauto.
+      assert (X ∉ dom Γ) as HA. {
+        assert (ok (Δ ++ [(X, bind_sub Q)] ++ Γ)) as HA by auto.
         apply ok_tail in HA.
         inversion HA...
       }
       forwards: notin_fv_wf_typ WfP HA.
       forwards: notin_fv_wf_typ WfQ HA.
-      replace (cv P `u` cset_set ({X}A `\`A X) {}N false)
-        with (cv P) by (destruct P; csetdec).
-      replace (cv P) with (subst_cset X (cv P) (cv P)) at 1.
+      replace (typ_cv P `u` cset_set ({X}A `\`A X) {}N false)
+        with (typ_cv P) by (destruct (typ_cv P); csetdec).
+      replace (typ_cv P) with (subst_cset X (typ_cv P) (typ_cv P)) at 1.
       2: {
         symmetry.
         apply subst_cset_fresh.
         destruct P; simpl in *; try fsetdec.
+        destruct v...
       }
-      apply (subcapt_transitivity (subst_cset X (cv P) (cv Q)))...
-      eenough (subcapt E _ _) as HE. {
-        rewrite_env (empty ++ (map (subst_tb X P) F ++ E)).
+      apply (subcapt_transitivity (subst_cset X (typ_cv P) (typ_cv Q)))...
+      eenough (Γ ⊢ₛ _ <: _) as HE. {
+        rewrite_env (∅ ++ (map (subst_tb X P) Δ ++ Γ)).
         apply subcapt_weakening; simpl_env...
       }
-      do 2 erewrite <- cv_subst_ct_correspondence by fsetdec.
+      do 2 erewrite <- typ_cv_subst_ct_correspondence by fsetdec.
       do 2 erewrite <- subst_ct_fresh by fsetdec.
       apply sub_implies_subcapt...
     + assert (x <> X) by fsetdec.
       binds_cases H.
-      * specialize (IHHsc X F Q E ltac:(trivial) ltac:(trivial) ltac:(trivial)).
+      * specialize (IHHsc X Δ Q Γ ltac:(trivial) ltac:(trivial) ltac:(trivial)).
         forwards: wf_typ_from_binds_sub H...
         eapply subcapt_tvar with (T := T)...
-        replace (cv T) with (subst_cset X (cv P) (cv T)).
+        replace (typ_cv T) with (subst_cset X (typ_cv P) (typ_cv T)).
         2: {
           symmetry; apply subst_cset_fresh.
-          assert (X `notin` dom E) as HA. {
-            assert (ok (F ++ [(X, bind_sub Q)] ++ E)) as HA by auto.
+          assert (X ∉ dom Γ) as HA. {
+            assert (ok (Δ ++ [(X, bind_sub Q)] ++ Γ)) as HA by auto.
             apply ok_tail in HA.
             inversion HA...
           }
           forwards: notin_fv_wf_typ H1 HA.
-          destruct T; simpl in *; fsetdec.
+          destruct T; simpl in *; try fsetdec.
+          destruct v...
         }
         apply IHHsc...
-      * assert (binds x (bind_sub (subst_tt X P T)) (map (subst_tb X P) F ++ E)) as HBnd by auto.
+      * assert (binds x (bind_sub (subst_tt X P T)) (map (subst_tb X P) Δ ++ Γ)) as HBnd by auto.
         eapply subcapt_tvar...
-        replace (cv (subst_tt X P T))
-          with (subst_cset X (cv P) (cv T)).
+        replace (typ_cv (subst_tt X P T))
+          with (subst_cset X (typ_cv P) (typ_cv T)).
         1: eapply IHHsc...
         1: {
-          destruct T; simpl...
-          - unfold subst_cset.
-            destruct_if...
-            exfalso;csetdec.
-          - unfold subst_cset.
-            destruct (a == X); destruct_set_mem X {a}A; try (exfalso;fsetdec).
-            2: simpl...
-            note (wf_typ_in E P); simpl; unfold cset_union; csetdec.
+          destruct T; unfold subst_cset; simpl...
+          destruct v; simpl.
+          2-6: destruct_if; [ exfalso; csetdec | reflexivity ].
+          destruct (a == X); destruct_set_mem X {a}A; try (exfalso;fsetdec).
+          2: simpl...
+          note (Γ ⊢ P wf); simpl; unfold cset_union; csetdec.
         }
-  - assert (wf_cset_in (map (subst_tb X P) F ++ E)
-                       (subst_cset X (cv P) (cset_set xs {}N b))) as ?WF. {
-      eapply wf_cset_in_subst_tb...
+  - assert ((map (subst_tb X P) Δ ++ Γ) ⊢ₛ
+                       (subst_cset X (typ_cv P) (cset_set xs {}N b)) wf) as ?WF. {
+      eapply wf_cset_subst_tb...
       constructor.
       - intros y yIn.
-        enough (wf_cset_in (F ++ [(X, bind_sub Q)] ++ E) (`cset_fvar` y)) as HA. {
+        enough ((Δ ++ [(X, bind_sub Q)] ++ Γ) ⊢ₛ (`cset_fvar` y) wf) as HA. {
           inversion HA...
         }
         specialize (H0 y yIn); simpl in H0...
       - intros y yIn.
-        enough (wf_cset_in (F ++ [(X, bind_sub Q)] ++ E) (`cset_fvar` y)) as HA. {
+        enough ((Δ ++ [(X, bind_sub Q)] ++ Γ) ⊢ₛ (`cset_fvar` y) wf) as HA. {
           inversion HA...
         }
         specialize (H0 y yIn); simpl in H0...
     }
-    assert (wf_cset_in (map (subst_tb X P) F ++ E)
-                       (subst_cset X (cv P) D)) as ?WF. {
-      eapply wf_cset_in_subst_tb...
+    assert ((map (subst_tb X P) Δ ++ Γ) ⊢ₛ
+                       (subst_cset X (typ_cv P) D) wf) as ?WF. {
+      eapply wf_cset_subst_tb...
     }
 
     unfold subst_cset at 1.
@@ -931,29 +908,30 @@ Proof with eauto using wf_env_subst_tb, wf_cset_in_subst_tb, wf_typ_in_subst_tb 
       apply subcapt_set; trivial.
       - intros y yIn.
         assert (X <> y) by notin_solve.
-        replace (`cset_fvar` y) with (subst_cset X (cv P) (`cset_fvar` y))...
+        replace (`cset_fvar` y) with (subst_cset X (typ_cv P) (`cset_fvar` y))...
         unfold subst_cset.
         destruct_set_mem X (singleton y)...
         exfalso; fsetdec.
       - (* Should we have a lemma that `cset_uvar` is not affected by subst? *)
         (* Looking at that chain, we probably should. *)
         destruct D; unfold subst_cset; destruct_if; destruct P; simpl; csetdec.
+        destruct v...
     }
 
     unfold AtomSet.F.For_all in H0.
 
     inversion H; subst.
-    assert (wf_cset_in (F ++ [(X, bind_sub Q)] ++ E) (cv P)) as HA. {
-      note (wf_env ([(X, bind_sub Q)] ++ E)) by eauto...
-      rewrite_env (empty ++ (F ++ [(X, bind_sub Q)]) ++ E).
-      apply wf_cset_in_weakening; simpl_env; [apply cv_wf|]...
+    assert ((Δ ++ [(X, bind_sub Q)] ++ Γ) ⊢ₛ (typ_cv P) wf) as HA. {
+      note (([(X, bind_sub Q)] ++ Γ) ⊢ wf) by eauto...
+      rewrite_env (∅ ++ (Δ ++ [(X, bind_sub Q)]) ++ Γ).
+      apply wf_cset_weakening; simpl_env; [apply cv_wf|]...
     }
     inversion HA; subst.
 
     rename fvars into cs', univ into b__c', fvars0 into ds, univ0 into b__d.
     unfold subst_cset in WF0 |- *.
     destruct_set_mem X cs'.
-    + rename select (_ = cv P) into EQ.
+    + rename select (_ = typ_cv P) into EQ.
       rewrite <- EQ in WF, WF0.
       csetsimpl.
       apply subcapt_set; trivial.
@@ -983,14 +961,14 @@ Proof with eauto using wf_env_subst_tb, wf_cset_in_subst_tb, wf_typ_in_subst_tb 
         apply subcapt_in...
         applys wf_cset_singleton_by_mem (ds `u`A xs `\`A X)...
       * cleanup_singleton_eq' x y x0.
-        rename select (_ = cv P) into EQ.
-        replace (`cset_fvar` y) with (subst_cset X (cv P) (`cset_fvar` y)).
+        rename select (_ = typ_cv P) into EQ.
+        replace (`cset_fvar` y) with (subst_cset X (typ_cv P) (`cset_fvar` y)).
         2: {
           unfold subst_cset; simpl.
           destruct_set_mem X (singleton y); (trivial || exfalso;fsetdec).
         }
         replace (cset_set (ds `union` cs' `remove` X) {}N (b__d || b__c'))
-          with (subst_cset X (cv P) (cset_set cs' {}N b__c')).
+          with (subst_cset X (typ_cv P) (cset_set cs' {}N b__c')).
         2: {
           unfold subst_cset; simpl.
           destruct_set_mem X cs'; [|exfalso;fsetdec].
@@ -1000,14 +978,14 @@ Proof with eauto using wf_env_subst_tb, wf_cset_in_subst_tb, wf_typ_in_subst_tb 
         (* rewrite EQ. *)
         eapply H1...
       * cleanup_singleton_eq' x y x0.
-        rename select (_ = cv P) into EQ.
-        replace (`cset_fvar` y) with (subst_cset X (cv P) (`cset_fvar` y)).
+        rename select (_ = typ_cv P) into EQ.
+        replace (`cset_fvar` y) with (subst_cset X (typ_cv P) (`cset_fvar` y)).
         2: {
           unfold subst_cset; simpl.
           destruct_set_mem X (singleton y); (trivial || exfalso;fsetdec).
         }
         replace (cset_set (ds `union` cs' `remove` X) {}N (b__d || b__c'))
-          with (subst_cset X (cv P) (cset_set cs' {}N b__c')).
+          with (subst_cset X (typ_cv P) (cset_set cs' {}N b__c')).
         2: {
           unfold subst_cset; simpl.
           destruct_set_mem X cs'; [|exfalso;fsetdec].
@@ -1015,14 +993,14 @@ Proof with eauto using wf_env_subst_tb, wf_cset_in_subst_tb, wf_typ_in_subst_tb 
           unfold cset_union; csetsimpl...
         }
         eapply H1...
-      * rename select (_ = cv P) into EQ.
-        replace (`cset_fvar` y) with (subst_cset X (cv P) (`cset_fvar` y)).
+      * rename select (_ = typ_cv P) into EQ.
+        replace (`cset_fvar` y) with (subst_cset X (typ_cv P) (`cset_fvar` y)).
         2: {
           unfold subst_cset; simpl.
           destruct_set_mem X (singleton y); (trivial || exfalso;fsetdec).
         }
         replace (cset_set (ds `union` cs' `remove` X) {}N (b__d || b__c'))
-          with (subst_cset X (cv P) (cset_set cs' {}N b__c')).
+          with (subst_cset X (typ_cv P) (cset_set cs' {}N b__c')).
         2: {
           unfold subst_cset; simpl.
           destruct_set_mem X cs'; [|exfalso;fsetdec].
@@ -1031,10 +1009,10 @@ Proof with eauto using wf_env_subst_tb, wf_cset_in_subst_tb, wf_typ_in_subst_tb 
         }
         eapply H1...
     + csetsimpl.
-      rename select (_ = cv P) into EQ.
+      rename select (_ = typ_cv P) into EQ.
       apply subcapt_set; trivial.
       2: {
-        forwards SpH1: H1 X X F Q E...
+        forwards SpH1: H1 X X Δ Q Γ...
         rewrite <- EQ in SpH1.
         unfold subst_cset in SpH1.
         find_and_destroy_set_mem; [|exfalso;fsetdec].
@@ -1051,40 +1029,40 @@ Proof with eauto using wf_env_subst_tb, wf_cset_in_subst_tb, wf_typ_in_subst_tb 
            rewrite <- EQ in WF; csetsimpl; applys wf_cset_singleton_by_mem yIn...
         -- cleanup_singleton_eq' x y x0.
            apply subcapt_in...
-           replace (`cset_fvar` y) with (subst_cset X (cv P) (`cset_fvar` y)).
-           eapply wf_cset_in_subst_tb...
+           replace (`cset_fvar` y) with (subst_cset X (typ_cv P) (`cset_fvar` y)).
+           eapply wf_cset_subst_tb...
            symmetry.
            apply subst_cset_fresh...
         -- cleanup_singleton_eq' x y x0.
-           replace (`cset_fvar` y) with (subst_cset X (cv P) (`cset_fvar` y)).
+           replace (`cset_fvar` y) with (subst_cset X (typ_cv P) (`cset_fvar` y)).
            2: {
              unfold subst_cset; simpl.
              destruct_set_mem X (`cset_fvar` y); (trivial || exfalso;fsetdec).
            }
-           replace (cset_set cs' {}N b__c') with (subst_cset X (cv P) (cset_set cs' {}N b__c')).
+           replace (cset_set cs' {}N b__c') with (subst_cset X (typ_cv P) (cset_set cs' {}N b__c')).
            2: {
              unfold subst_cset; simpl.
              destruct_set_mem X cs'; (trivial||exfalso;fsetdec).
            }
            eapply H1...
         -- cleanup_singleton_eq' x y x0.
-           replace (`cset_fvar` y) with (subst_cset X (cv P) (`cset_fvar` y)).
+           replace (`cset_fvar` y) with (subst_cset X (typ_cv P) (`cset_fvar` y)).
            2: {
              unfold subst_cset; simpl.
              destruct_set_mem X (`cset_fvar` y); (trivial || exfalso;fsetdec).
            }
-           replace (cset_set cs' {}N b__c') with (subst_cset X (cv P) (cset_set cs' {}N b__c')).
+           replace (cset_set cs' {}N b__c') with (subst_cset X (typ_cv P) (cset_set cs' {}N b__c')).
            2: {
              unfold subst_cset; simpl.
              destruct_set_mem X cs'; (trivial||exfalso;fsetdec).
            }
            eapply H1...
-        -- replace (`cset_fvar` y) with (subst_cset X (cv P) (`cset_fvar` y)).
+        -- replace (`cset_fvar` y) with (subst_cset X (typ_cv P) (`cset_fvar` y)).
            2: {
              unfold subst_cset; simpl.
              destruct_set_mem X (`cset_fvar` y); (trivial || exfalso;fsetdec).
            }
-           replace (cset_set cs' {}N b__c') with (subst_cset X (cv P) (cset_set cs' {}N b__c')).
+           replace (cset_set cs' {}N b__c') with (subst_cset X (typ_cv P) (cset_set cs' {}N b__c')).
            2: {
              unfold subst_cset; simpl.
              destruct_set_mem X cs'; (trivial||exfalso;fsetdec).
@@ -1093,7 +1071,7 @@ Proof with eauto using wf_env_subst_tb, wf_cset_in_subst_tb, wf_typ_in_subst_tb 
       * destruct_union_mem yIn.
         2: exfalso...
         rename H1 into H1'.
-        forwards H1: (>> H1' X XIn X F Q E)...
+        forwards H1: (>> H1' X XIn X Δ Q Γ)...
         move H1 before H1'; clear H1'.
         unfold subst_cset at 1 in H1.
         destruct_set_mem X {X}A; [|exfalso;fsetdec].
@@ -1106,58 +1084,54 @@ Proof with eauto using wf_env_subst_tb, wf_cset_in_subst_tb, wf_typ_in_subst_tb 
 
         replace (ds `u`A {X}A `\`A X) with ds in H1 by fsetdec.
 
-        enough (subcapt (map (subst_tb X P) F ++ E)
-                         (`cset_fvar` y)
+        enough ((map (subst_tb X P) Δ ++ Γ) ⊢ₛ
+                         (`cset_fvar` y) <:
                          (cset_set ds {}N b__d)) as HAA. {
           eapply subcapt_transitivity...
         }
         eapply subcapt_in...
         forwards (? & ?): subcapt_regular H1.
-        inversion select (wf_cset_in _ (cset_set ds _ _)); subst...
+        inversion select (_ ⊢ₛ (cset_set ds _ _) wf); subst...
+        eapply wf_cset_singleton_by_mem...
+        repeat rewrite dom_concat in *; repeat rewrite dom_map in *; simpl in *.
         admit.
 Admitted.
 
 (* (* ********************************************************************** *) *)
 (* (** ** Narrowing and transitivity (3) *) *)
 
-Lemma subst_cset_across_subcapt : forall E x C D C0 A,
-  wf_env E ->
-  wf_cset E A C0 ->
-  A `subset` dom E ->
-  subcapt E C D ->
-  subcapt E (subst_cset x C C0) (subst_cset x D C0).
+Lemma subst_cset_across_subcapt : forall Γ x C D C0,
+  Γ ⊢ wf ->
+  Γ ⊢ₛ C0 wf ->
+  Γ ⊢ₛ C <: D ->
+  Γ ⊢ₛ (subst_cset x C C0) <: (subst_cset x D C0).
 Proof with eauto with fsetdec.
-  intros * WfEnv Wf Subset Sub.
-  assert (wf_cset_in E (subst_cset x C C0)). {
+  intros * WfEnv Wf Sub.
+  assert (Γ ⊢ₛ (subst_cset x C C0) wf). {
     unfold subst_cset.
-    destruct_set_mem x (`cset_fvars` C0).
-    2: eapply wf_cset_set_weakening...
+    destruct_set_mem x (`cset_fvars` C0)...
     apply wf_cset_union...
-    apply wf_cset_remove_fvar.
-    eapply wf_cset_set_weakening...
+    apply wf_cset_remove_fvar...
   }
-  assert (wf_cset_in E (subst_cset x D C0)). {
+  assert (Γ ⊢ₛ (subst_cset x D C0) wf). {
     unfold subst_cset.
-    destruct_set_mem x (`cset_fvars` C0).
-    2: eapply wf_cset_set_weakening...
+    destruct_set_mem x (`cset_fvars` C0)...
     apply wf_cset_union...
-    apply wf_cset_remove_fvar.
-    eapply wf_cset_set_weakening...
+    apply wf_cset_remove_fvar...
   }
 
   inversion Wf; subst.
   rename fvars into zs.
 
-  note (wf_cset_in E C).
+  note (Γ ⊢ₛ C wf).
   rename fvars into cs.
 
-  note (wf_cset_in E D).
+  note (Γ ⊢ₛ D wf).
   rename fvars into ds.
 
   unfold subst_cset in H0, H |- *; destruct_set_mem x zs.
   2: {
     eapply subcapt_reflexivity...
-    fsetdec.
   }
 
   dependent induction Sub.
@@ -1170,14 +1144,16 @@ Proof with eauto with fsetdec.
       destruct (AtomSet.F.union_1 yIn).
       * assert (y = x0) by fsetdec; subst...
       * apply wf_concrete_cset...
-        fsetdec.
+        2: fsetdec.
+        intros z zIn...
     + csetdec.
   - csetsimpl.
     apply subcapt_set...
     intros y yIn.
     apply subcapt_in...
     apply wf_concrete_cset...
-    fsetdec.
+    2: fsetdec.
+    intros z zIn...
   - csetsimpl.
     apply subcapt_set...
     2: csetdec.
@@ -1186,7 +1162,8 @@ Proof with eauto with fsetdec.
     2: {
       apply subcapt_in...
       apply wf_concrete_cset...
-      fsetdec.
+      2: fsetdec.
+      intros z zIn...
     }
     rename select (y `in`A _) into yIn.
     apply AtomSetFacts.singleton_iff in yIn; symmetry in yIn; subst.
@@ -1196,7 +1173,8 @@ Proof with eauto with fsetdec.
     + intros z zIn.
       apply subcapt_in...
       apply wf_concrete_cset...
-      fsetdec.
+      2: fsetdec.
+      intros w wIn...
     + csetdec.
   - csetsimpl.
     apply subcapt_set...
@@ -1206,7 +1184,8 @@ Proof with eauto with fsetdec.
     2: {
       apply subcapt_in...
       apply wf_concrete_cset...
-      fsetdec.
+      2: fsetdec.
+      intros z zIn...
     }
     rename select (y `in`A _) into yIn.
     apply AtomSetFacts.singleton_iff in yIn; symmetry in yIn; subst.
@@ -1216,7 +1195,8 @@ Proof with eauto with fsetdec.
     + intros z zIn.
       apply subcapt_in...
       apply wf_concrete_cset...
-      fsetdec.
+      2: fsetdec.
+      intros w wIn...
     + csetdec.
   - csetsimpl.
     apply subcapt_set...
@@ -1226,7 +1206,8 @@ Proof with eauto with fsetdec.
     2: {
       apply subcapt_in...
       apply wf_concrete_cset...
-      fsetdec.
+      2: fsetdec.
+      intros z zIn...
     }
     apply (subcapt_transitivity (cset_set ds {}N univ1))...
 
@@ -1234,22 +1215,23 @@ Proof with eauto with fsetdec.
     + intros z zIn.
       apply subcapt_in...
       apply wf_concrete_cset...
-      fsetdec.
+      2: fsetdec.
+      intros w wIn...
     + csetdec.
 Qed.
 
-Lemma subcapt_strengthening : forall G F E C1 C2,
-  ok (G ++ F ++ E) ->
-  wf_env (G ++ E) ->
-  wf_cset_in (G ++ E) C1 ->
-  wf_cset_in (G ++ E) C2 ->
-  subcapt (G ++ F ++ E) C1 C2 ->
-  subcapt (G ++ E) C1 C2.
+Lemma subcapt_strengthening : forall Δ Θ Γ C1 C2,
+  ok (Δ ++ Θ ++ Γ) ->
+  (Δ ++ Γ) ⊢ wf ->
+  (Δ ++ Γ) ⊢ₛ C1 wf ->
+  (Δ ++ Γ) ⊢ₛ C2 wf ->
+  (Δ ++ Θ ++ Γ) ⊢ₛ C1 <:  C2 ->
+  (Δ ++ Γ) ⊢ₛ C1 <: C2.
 Proof with eauto.
   intros * Ok WfE Wf1 Wf2 Sc.
   dependent induction Sc...
   - inversion Wf1; subst; cbv [allbound] in *...
-    specialize (H4 x ltac:(fsetdec)) as [Tx Hbinds].
+    specialize (H3 x ltac:(fsetdec)) as [Tx Hbinds].
     destruct Hbinds...
     * assert (Tx = T). {
         eapply binds_weaken in H0...
@@ -1266,7 +1248,7 @@ Proof with eauto.
       unshelve epose proof (binds_unique _ _ _ _ H H0)...
       inversion H1...
   - inversion Wf1; subst; cbv [allbound] in *...
-    specialize (H4 x ltac:(fsetdec)) as [Tx Hbinds].
+    specialize (H3 x ltac:(fsetdec)) as [Tx Hbinds].
     destruct Hbinds...
     * exfalso.
       eapply binds_weaken in H0...
@@ -1290,67 +1272,72 @@ Proof with eauto.
       inversion Wf1; subst.
       eapply wf_concrete_cset...
       -- intros z zIn; assert (z = a) by (clear - zIn; fsetdec); subst...
-      -- rewrite dom_concat in H10 |- *.
+      -- rewrite dom_concat in H9 |- *.
          fsetdec.
 Qed.
 
-Lemma subcapt_widening_univ : forall X F E P Q C,
-  ok (F ++ [(X, bind_sub Q)] ++ E) ->
-  subcapt (F ++ [(X, bind_sub P)] ++ E) {*} C ->
-  sub E P Q ->
-  subcapt (F ++ [(X, bind_sub Q)] ++ E) {*} C.
+Lemma subcapt_widening_univ : forall X Δ Γ P Q C,
+  ok (Δ ++ [(X, bind_sub Q)] ++ Γ) ->
+  (Δ ++ [(X, bind_sub P)] ++ Γ) ⊢ₛ {*} <: C ->
+  Γ ⊢ P <: Q ->
+  (Δ ++ [(X, bind_sub Q)] ++ Γ) ⊢ₛ {*} <: C.
 Proof with eauto using wf_cset_narrowing.
   intros * Ok Sc Sub.
   dependent induction Sc...
 Qed.
 
-Lemma subcapt_widening_typ_univ : forall X F E P Q C,
-  ok (F ++ [(X, bind_typ Q)] ++ E) ->
-  subcapt (F ++ [(X, bind_typ P)] ++ E) {*} C ->
-  sub E P Q ->
-  subcapt (F ++ [(X, bind_typ Q)] ++ E) {*} C.
+Lemma subcapt_widening_typ_univ : forall X Δ Γ P Q C,
+  ok (Δ ++ [(X, bind_typ Q)] ++ Γ) ->
+  (Δ ++ [(X, bind_typ P)] ++ Γ) ⊢ₛ {*} <: C ->
+  Γ ⊢ P <: Q ->
+  (Δ ++ [(X, bind_typ Q)] ++ Γ) ⊢ₛ {*} <: C.
 Proof with eauto using wf_cset_narrowing_typ.
   intros * Ok Sc Sub.
   dependent induction Sc...
 Qed.
 
-Lemma univ_supercapt_inversion : forall E C,
-  subcapt E {*} C ->
-  `* in` C.
+Lemma univ_supercapt_inversion : forall Γ C,
+  Γ ⊢ₛ {*} <: C ->
+  * ∈ C.
 Proof with eauto.
   intros * Hsc.
   dependent induction Hsc...
 Qed.
 
-Lemma subcapt_univ_through_subst_cb : forall F E x u P T,
-  wf_cset_in (F ++ [(x, bind_typ (typ_capt (free_for_cv u) P))] ++ E) (cv T) ->
-  subcapt (map (subst_cb x (free_for_cv u)) F ++ E) {*} (cv (subst_ct x (free_for_cv u) T)) ->
-  subcapt (F ++ [(x, bind_typ (typ_capt (free_for_cv u) P))] ++ E) {*} (cv T).
+(* TODO: move to CCsub_Lemmas.v
+typ_cv_free_never_universal *)
+
+Lemma subcapt_univ_through_subst_cb : forall Δ Γ x u P T,
+  (Δ ++ [(x, bind_typ (exp_cv u # P))] ++ Γ) ⊢ₛ (typ_cv T) wf ->
+  (map (subst_cb x (exp_cv u)) Δ ++ Γ) ⊢ₛ {*} <: (typ_cv (subst_ct x (exp_cv u) T)) ->
+  (Δ ++ [(x, bind_typ (typ_capt (exp_cv u) P))] ++ Γ) ⊢ₛ {*} <: (typ_cv T).
 Proof with eauto.
   intros * Wf ScUniv.
-
   forwards UIn: univ_supercapt_inversion ScUniv.
-  destruct T; simpl in *; try congruence.
+  destruct T; simpl in *; try congruence; unfold subst_cset in UIn.
+  1: destruct v...
   unfold subst_cset in UIn.
-  forwards: cv_free_never_universal u.
+  (* forwards: cv_free_never_universal u. *)
   find_and_destroy_set_mem.
-  + destruct (free_for_cv u).
-    destruct b; try congruence.
+  + destruct (exp_cv u).
+    destruct b; try congruence...
     inversion Wf; subst.
     csetsimpl.
     apply subcapt_in_univ; trivial.
+    (* REVIEW: unsolvable? previously used cv_never_universal which is not true anymore *)
+    admit.
   + apply subcapt_in_univ; trivial.
-Qed.
+Admitted.
 
-Lemma subcapt_univ_through_subst_tb : forall F E Z P T,
-  wf_typ_in (F ++ [(Z, bind_sub P)] ++ E) T ->
-  wf_typ_in E P ->
-  subcapt (map (subst_tb Z P) F ++ E) {*} (cv (subst_tt Z P T)) ->
-  subcapt (F ++ [(Z, bind_sub P)] ++ E) {*} (cv T) \/
-    (Z `in` (`cset_fvars` (cv T)) /\ subcapt E {*} (cv P)).
+Lemma subcapt_univ_through_subst_tb : forall Δ Γ Z P T,
+  (Δ ++ [(Z, bind_sub P)] ++ Γ) ⊢ T wf ->
+  Γ ⊢ P wf ->
+  (map (subst_tb Z P) Δ ++ Γ) ⊢ₛ {*} <: typ_cv (subst_tt Z P T) ->
+  (Δ ++ [(Z, bind_sub P)] ++ Γ) ⊢ₛ {*} <: typ_cv T
+    \/ (Z ∈ (`cset_fvars` (typ_cv T))
+          /\ Γ ⊢ₛ {*} <: typ_cv P).
 Proof with eauto.
   intros * WfT WfP ScUniv.
-
   forwards: univ_supercapt_inversion ScUniv.
   inversion WfT; subst; simpl in *; simpl_env in *; try congruence.
   - destruct (X == Z); subst.
@@ -1364,14 +1351,12 @@ Proof with eauto.
     1: {
       left.
       apply subcapt_in_univ; trivial.
-      apply (wf_cset_adapt H0).
-      simpl_env; fsetdec.
     }
     unfold subst_cset in H.
     find_and_destroy_set_mem; try congruence.
-    assert (wf_cset_in E (cv P)) as WfCvP by (eapply cv_wf; eauto).
+    assert (Γ ⊢ₛ (typ_cv P) wf) as WfCvP by (eapply cv_wf; eauto).
     inversion WfCvP; subst.
-    rename select (_ = cv P) into EQ; rewrite <- EQ in *.
+    rename select (_ = typ_cv P) into EQ; rewrite <- EQ in *.
     unfold cset_union in H.
     destruct univ; simpl in *; try congruence.
     right; split...
